nit

examples/dsls/mini_steel/Pulse.Steel.Wrapper.fsti
@@ -96,6 +96,9 @@ val bind_sttg
   (e2:(x:a -> stt_ghost b opened (post1 x) post2))
   : stt_ghost b opened pre1 post2
 
+type non_informative_witness (a:Type u#a) =
+  x:Ghost.erased a -> y:a{y == Ghost.reveal x}
+
 inline_for_extraction
 val bind_stt_atomic_ghost
   (#a:Type u#a) (#b:Type u#b)
@@ -103,7 +106,7 @@ val bind_stt_atomic_ghost
   (#pre1:vprop) (#post1:a -> vprop) (#post2:b -> vprop)
   (e1:stt_atomic a opened pre1 post1)
   (e2:(x:a -> stt_ghost b opened (post1 x) post2))
-  (reveal_b:(x:Ghost.erased b -> y:b{y == Ghost.reveal x}))
+  (reveal_b:non_informative_witness b)
   : stt_atomic b opened pre1 post2
 
 inline_for_extraction
@@ -113,7 +116,7 @@ val bind_stt_ghost_atomic
   (#pre1:vprop) (#post1:a -> vprop) (#post2:b -> vprop)
   (e1:stt_ghost a opened pre1 post1)
   (e2:(x:a -> stt_atomic b opened (post1 x) post2))
-  (reveal_a:(x:Ghost.erased a -> y:a{y == Ghost.reveal x}))
+  (reveal_a:non_informative_witness a)
   : stt_atomic b opened pre1 post2
 
 inline_for_extraction
